Weidenbach_Book/IsaSAT_Watch_List_SML.thy
@@ -2,6 +2,178 @@ theory IsaSAT_Watch_List_SML
   imports Watched_Literals.Array_Array_List64 IsaSAT_Watch_List IsaSAT_Literals_SML
 begin
 
+definition watcher_enc where
+  \<open>watcher_enc = {(n, (L, b)). \<exists>L'. (L', L) \<in> unat_lit_rel \<and>
+      n = uint64_of_uint32 L' + (if b then 1 << 32 else 0)}\<close>
+
+definition take_only_lower32 :: \<open>uint64 \<Rightarrow> uint64\<close> where
+  [code del]: \<open>take_only_lower32 n = n AND ((1 << 32) - 1)\<close>
+
+
+lemma nat_less_numeral_unfold: fixes n :: nat shows
+  "n < numeral w \<longleftrightarrow> n = pred_numeral w \<or> n < pred_numeral w"
+by(auto simp add: numeral_eq_Suc)
+
+lemma bin_nth2_32_iff: \<open>bin_nth 4294967295 na \<longleftrightarrow> na < 32\<close>
+  by (auto simp: bin_nth_Bit1 bin_nth_Bit0 nat_less_numeral_unfold)
+
+lemma take_only_lower32_le_uint32_max:
+  \<open>nat_of_uint64 n \<le> uint32_max \<Longrightarrow> take_only_lower32 n = n\<close>
+  unfolding take_only_lower32_def
+  apply transfer
+  by (auto intro!: and_eq_bits_eqI dest: unat_le_uint32_max_no_bit_set
+    intro!: bin_nth2_32_iff[THEN iffD2])
+
+
+lemma uint32_of_uint64_uint64_of_uint32[simp]: \<open>uint32_of_uint64 (uint64_of_uint32 n) = n\<close>
+  by (auto simp: uint64_of_uint32_def uint32_of_uint64_def
+    nat_of_uint64_uint64_of_nat_id nat_of_uint32_le_uint32_max nat_of_uint32_le_uint64_max)
+
+lemma take_only_lower32_le_uint32_max_ge_uint32_max:
+  \<open>nat_of_uint64 n \<le> uint32_max \<Longrightarrow> nat_of_uint64 m \<ge> uint32_max \<Longrightarrow> take_only_lower32 m = 0 \<Longrightarrow>
+    take_only_lower32 (n + m) = n\<close>
+  unfolding take_only_lower32_def
+  apply transfer
+  subgoal for m n
+    using ex_rbl_word64_le_uint32_max[of m] ex_rbl_word64_ge_uint32_max[of n]
+    apply (auto intro: and_eq_bits_eqI simp: bin_nth2_32_iff word_add_rbl
+      dest: unat_le_uint32_max_no_bit_set)
+    apply (rule word_bl.Rep_inject[THEN iffD1])
+    apply (auto simp del: word_bl.Rep_inject simp: bl_word_and word_add_rbl
+      split!: if_splits)
+    done
+  done
+
+lemma take_only_lower32_1_32: \<open>take_only_lower32 (1 << 32) = 0\<close>
+  unfolding take_only_lower32_def
+  by transfer (auto simp: )
+
+lemma nat_of_uint64_1_32: \<open>nat_of_uint64 (1 << 32) = uint32_max + 1\<close>
+  unfolding uint32_max_def
+  by transfer auto
+
+lemma watcher_enc_extract_blit:
+  assumes \<open>(n, (L, b)) \<in> watcher_enc\<close>
+  shows \<open>(uint32_of_uint64 (take_only_lower32 n), L) \<in> unat_lit_rel\<close>
+  using assms
+  by (auto simp: watcher_enc_def take_only_lower32_le_uint32_max nat_of_uint64_uint64_of_uint32
+    nat_of_uint32_le_uint32_max nat_of_uint64_1_32 take_only_lower32_1_32
+      take_only_lower32_le_uint32_max_ge_uint32_max)
+
+fun blit_of where
+  \<open>blit_of (_, (L, _)) = L\<close>
+
+fun blit_of_code where
+  \<open>blit_of_code (n, bL) = uint32_of_uint64 (take_only_lower32 bL)\<close>
+
+fun is_marked_binary where
+  \<open>is_marked_binary (_, (_, b)) = b\<close>
+
+fun is_marked_binary_code :: \<open>_ \<times> uint64 \<Rightarrow> bool\<close> where
+  [code del]: \<open>is_marked_binary_code (_, bL) = (bL AND ((2 :: uint64)^32) \<noteq> 0)\<close>
+
+lemma [code]:
+  \<open>is_marked_binary_code (n, bL) = (bL AND 4294967296 \<noteq> 0)\<close>
+  by auto
+
+lemma AND_2_32_bool:
+  \<open>nat_of_uint64 n \<le> uint32_max \<Longrightarrow> n + (1 << 32) AND 4294967296 = 4294967296\<close>
+  apply transfer
+  subgoal for n
+    using ex_rbl_word64_ge_uint32_max[of \<open>1 << 32\<close>] ex_rbl_word64_le_uint32_max[of n]
+    apply (auto intro: and_eq_bits_eqI simp: bin_nth2_32_iff word_add_rbl
+      dest: unat_le_uint32_max_no_bit_set)
+    apply (rule word_bl.Rep_inject[THEN iffD1])
+    apply (auto simp del: word_bl.Rep_inject simp: bl_word_and word_add_rbl
+      split!: if_splits)
+    done
+  done
+
+lemma watcher_enc_extract_bool_True:
+  assumes \<open>(n, (L, True)) \<in> watcher_enc\<close>
+  shows \<open>n AND 4294967296 = 4294967296\<close>
+  using assms
+  by (auto simp: watcher_enc_def take_only_lower32_le_uint32_max nat_of_uint64_uint64_of_uint32
+    nat_of_uint32_le_uint32_max nat_of_uint64_1_32 take_only_lower32_1_32 AND_2_32_bool
+      take_only_lower32_le_uint32_max_ge_uint32_max)
+
+lemma le_uint32_max_AND2_32_eq0: \<open>nat_of_uint64 n \<le> uint32_max \<Longrightarrow> n AND 4294967296 = 0\<close>
+  apply transfer
+  subgoal for n
+    using ex_rbl_word64_le_uint32_max[of n]
+    apply (auto intro!: )
+    apply (rule word_bl.Rep_inject[THEN iffD1])
+    apply (auto simp del: word_bl.Rep_inject simp: bl_word_and word_add_rbl
+      split!: if_splits)
+    done
+  done
+
+lemma watcher_enc_extract_bool_False:
+  assumes \<open>(n, (L, False)) \<in> watcher_enc\<close>
+  shows \<open>(n AND 4294967296 = 0)\<close>
+  using assms
+  by (auto simp: watcher_enc_def take_only_lower32_le_uint32_max nat_of_uint64_uint64_of_uint32
+    nat_of_uint32_le_uint32_max nat_of_uint64_1_32 take_only_lower32_1_32 AND_2_32_bool
+      take_only_lower32_le_uint32_max_ge_uint32_max le_uint32_max_AND2_32_eq0)
+
+
+lemma watcher_enc_extract_bool:
+  assumes \<open>(n, (L, b)) \<in> watcher_enc \<close>
+  shows \<open>b \<longleftrightarrow> (n AND 4294967296 \<noteq> 0)\<close>
+  using assms
+  supply [[show_sorts]]
+  by (cases b)
+   (auto dest!: watcher_enc_extract_bool_False watcher_enc_extract_bool_True)
+
+definition watcher_of :: \<open>nat \<times> (nat literal \<times> bool) \<Rightarrow> _\<close> where
+  [simp]: \<open>watcher_of = id\<close>
+
+definition watcher_of_code :: \<open>nat \<times> uint64 \<Rightarrow> nat \<times> (uint32 \<times> bool)\<close> where
+  \<open>watcher_of_code = (\<lambda>(a, b). (a, (blit_of_code (a, b), is_marked_binary_code (a, b))))\<close>
+
+
+definition watcher_of_fast_code :: \<open>uint64 \<times> uint64 \<Rightarrow> uint64 \<times> (uint32 \<times> bool)\<close> where
+  \<open>watcher_of_fast_code = (\<lambda>(a, b). (a, (blit_of_code (a, b), is_marked_binary_code (a, b))))\<close>
+
+
+definition to_watcher :: \<open>nat \<Rightarrow> nat literal \<Rightarrow> bool \<Rightarrow> _\<close> where
+  [simp]: \<open>to_watcher n L b = (n, (L, b))\<close>
+
+definition to_watcher_code :: \<open>nat \<Rightarrow> uint32 \<Rightarrow> bool \<Rightarrow> nat \<times> uint64\<close> where
+  [code del]:
+    \<open>to_watcher_code = (\<lambda>a L b. (a, uint64_of_uint32 L OR (if b then 1 << 32 else (0 :: uint64))))\<close>
+
+
+lemma to_watcher_code[code]:
+  \<open>to_watcher_code a L b = (a, uint64_of_uint32 L OR (if b then 4294967296 else (0 :: uint64)))\<close>
+  by (auto simp: shiftl_integer_conv_mult_pow2 to_watcher_code_def shiftl_t2n_uint64)
+
+lemma OR_int64_0[simp]: \<open>A OR (0 :: uint64) = A\<close>
+  by transfer auto
+
+lemma OR_132_is_sum:
+  \<open>nat_of_uint64 n \<le> uint32_max \<Longrightarrow> n OR (1 << 32) = n + (1 << 32)\<close>
+  apply transfer
+  subgoal for n
+    using ex_rbl_word64_le_uint32_max[of n]
+    apply (auto intro: and_eq_bits_eqI simp: bin_nth2_32_iff word_add_rbl
+      dest: unat_le_uint32_max_no_bit_set)
+    apply (rule word_bl.Rep_inject[THEN iffD1])
+    by (auto simp del: word_bl.Rep_inject simp: bl_word_or word_add_rbl
+      split!: if_splits)
+  done
+
+definition to_watcher_fast where
+ [simp]: \<open>to_watcher_fast = to_watcher\<close>
+
+definition to_watcher_fast_code :: \<open>uint64 \<Rightarrow> uint32 \<Rightarrow> bool \<Rightarrow> uint64 \<times> uint64\<close> where
+  \<open>to_watcher_fast_code = (\<lambda>a L b. (a, uint64_of_uint32 L OR (if b then 1 << 32 else (0 :: uint64))))\<close>
+
+
+lemma take_only_lower_code[code]:
+  \<open>take_only_lower32 n = n AND 4294967295\<close>
+  by (auto simp: take_only_lower32_def shiftl_t2n_uint64)
+
 type_synonym watched_wl = \<open>((nat \<times> uint64) array_list) array\<close>
 type_synonym watched_wl_uint32 = \<open>((uint64 \<times> uint64) array_list64) array\<close>
 
